\renewcommand{\vec}[1]{\mathbf{#1}}
\newcommand{\half}{\frac{1}{2}}
\newcommand{\loss}{\Delta\left(\vec{y}, \vec{y}_i\right)}

% Traditional SVM Equation
\def\svmEquation
{
\begin{align}
    \min_\vec{w} & \half \vec{w} \cdot \vec{w} + C\sum_{i=1}^n\xi_i \\
    \text{s.t. } & \forall i \xi_i \ge 0 \nonumber \\
                 & \forall i y_i \left(\vec{w} \cdot \vec{x}_i + b\right) \ge 1 - \xi_i \nonumber
\end{align}
}

% Traditional SVM Dual
\def\traditionalDual
{
\begin{align}
    \max_\alpha & \sum_{i=1}^n \alpha_i - \half \sum_{i=1}^n \sum_{j=1}^n \alpha_i \alpha_j
    y_i y_j K\left(\vec{x}_i, \vec{x}_j\right) \\
    \text{s.t. } & \sum_{i=1}^n y_i \alpha_i = 0 \nonumber \\
    & 0 \le \alpha_i \le C \nonumber
\end{align}
}

% Fuzzy SVM Equation
\def\fuzzySvmEquation
{
\begin{align}
    \min_\vec{w} & \half \vec{w} \cdot \vec{w} + C\sum_{i=1}^n \alert{s_i} \xi_i \\
    \text{s.t. } & \forall i \xi_i \ge 0 \nonumber \\
                 & \forall i y_i \left(\vec{w} \cdot \vec{x}_i + b\right) \ge 1 - \xi_i \nonumber
\end{align}
}

% Fuzzy SVM Dual
\def\fuzzyDual
{
\begin{align}
    \max_\alpha & \sum_{i=1}^n \alpha_i - \half \sum_{i=1}^n \sum_{j=1}^n \alpha_i \alpha_j
    y_i y_j K\left(\vec{x}_i, \vec{x}_j\right) \\
    \text{s.t. } & \sum_{i=1}^n y_i \alpha_i = 0 \nonumber \\
    & 0 \le \alpha_i \le \alert{s_i} C \nonumber
\end{align}
}

\def\struckDiscriminant
{
    \begin{align}
        \vec{y}_t = \argmax_{\vec{y} \in \mathcal{Y}} F\left(\vec{x}_t^{\vec{p}_{t-1}}, \vec{y}\right)
    \end{align}
}

\def\struckEquation
{
    \begin{align}
        \label{eq:struck_svm}
        \min_\vec{w} & \half \vec{w} \cdot \vec{w} + C \sum_{i=1}^n \xi_i \\
        \text{s.t. } & \forall i : \xi_i \ge 0 \nonumber \\
        & \forall i : \forall \vec{y} \ne \vec{y}_i : \vec{w} \cdot \delta \vec{\Phi}_i(\vec{y}) \ge \loss - \xi_i \nonumber
    \end{align}
}

\def\struckDualAlpha
{
    \begin{align}
        \label{eq:struck_dual_alpha}
        \max_\alpha & \sum_{i,\vec{y} \ne \vec{y}_i} \loss \alpha_i^\vec{y} - \half
        \sum_{\substack{i, \vec{y} \ne \vec{y}_i \\ j, \vec{y} \ne \vec{y}_j}} \alpha_i^\vec{y}
        \alpha_j^\vec{\bar{y}} \delta \vec{\Phi}_i( \vec{y} ) \cdot \delta \vec{\Phi}_j(
        \vec{\bar{y}} ) \\
        \text{s.t. } & \forall i, \forall \vec{y} \ne \vec{y}_i : \alpha_i^\vec{y} \ge 0 \nonumber \\
        & \forall i : \sum_{\vec{y} \ne \vec{y}_i} \alpha_i^\vec{y} \le C \nonumber
    \end{align}
}

\def\struckDualBeta
{
    \begin{align}
        \label{eq:struck_dual_beta}
        \max_\beta & - \sum_{i, \vec{y}} \loss \beta_i^\vec{y} - \half \sum_{i, \vec{y}, j,
        \vec{\bar{y}}} \beta_i^\vec{y} \beta_j^\vec{\bar{y}} \vec{\Phi} \left( \vec{x}_i, \vec{y}
        \right) \cdot \vec{\Phi} \left( \vec{x}_j, \vec{\bar{y}} \right) \\
        \text{s.t. } & \forall i, \forall \vec{y} : \beta_i^\vec{y} \le \begin{cases}
            0 & \vec{y} \ne \vec{y}_i \\
            C & \vec{y} = \vec{y}_i
        \end{cases} \nonumber \\
        & \forall i : \sum_\vec{y} \beta_i^\vec{y} = 0 \nonumber
    \end{align}
}

\def\struckNewDiscriminant
{
    \[ F(\vec{x}, \vec{y}) = \sum_{j, \vec{\bar{y}}} \beta_j^\vec{\bar{y}} \vec{\Phi} \left( \vec{x}_i, \vec{y}
        \right) \cdot \vec{\Phi} \left( \vec{x}_j, \vec{\bar{y}} \right) \]
}

\def\struckGradients
{
    \begin{align}
        g_i(\vec{y}) &= -\loss - \sum_{j, \vec{\bar{y}}} \beta_j^\vec{\bar{y}} \vec{\Phi} \left( \vec{x}_i, \vec{y}
        \right) \cdot \vec{\Phi} \left( \vec{x}_j, \vec{\bar{y}} \right) \nonumber \\
        &= -\loss -F \left( \vec{x}_i, \vec{y} \right)
    \end{align}
}

\def\struckWeightChange
{
    \begin{align}
        \label{eq:struck_weights}
        \vec{\bar{w}} &= \vec{w} - \beta_r^\vec{y} \vec{\Phi} \left( \vec{x}_r, \vec{y} \right) +
        \beta_r^\vec{y} \vec{\Phi} \left( \vec{x}_r, \vec{y}_r \right) \\
        \|\Delta \vec{w}\|^2 &= \beta_r^{\vec{y}^2} [ \vec{\Phi} \left( \vec{x}_r, \vec{y}
        \right) \cdot \vec{\Phi} \left( \vec{x}_r, \vec{y} \right) + \nonumber \\
        & \vec{\Phi} \left( \vec{x}_r,
        \vec{y}_r \right) \cdot \vec{\Phi} \left( \vec{x}_r, \vec{y}_r \right) - 2 \vec{\Phi} \left(
        \vec{x}_r, \vec{y} \right) \cdot \vec{\Phi} \left( \vec{x}_r, \vec{y}_r \right) ] \nonumber
    \end{align}
}

\def\struckSmo
{
    \begin{algorithm}%[H]
        \DontPrintSemicolon
        \KwIn{\(i, \vec{y}_-, \vec{y}_+\)}
        \Begin(SMO Step)
        {
            \(\lambda^u = \frac{g_i(\vec{y}_+) - g_i(\vec{y}_-)}{K_{++} + K_{--} -2K_{+-}}\)\;
            \(\lambda = max(0, min(\lambda^u, C \delta (\vec{y}_+, \vec{y}_-) - \beta_i^{\vec{y}_+})) \)\;
            \(\beta_i^{\vec{y}_+} \gets \beta_i{\vec{y}_+} + \lambda\)\;
            \(\beta_i^{\vec{y}_-} \gets \beta_i{\vec{y}_-} - \lambda\)\;
            \ForEach{\((\vec{x}_j, \vec{y}) \in \mathcal{S}\)}
            {
                \(K_0 = \vec{\Phi} (\vec{x}_j, \vec{y}) \cdot \vec{\Phi} (\vec{x}_i, \vec{y}_+)\)\;
                \(K_1 = \vec{\Phi} (\vec{x}_j, \vec{y}) \cdot \vec{\Phi} (\vec{x}_i, \vec{y}_-)\)\;
                \(g_j(\vec{y}) \gets g_j(\vec{y}) - \lambda (K_0 - K_1)\)\;
            }
        }
    \end{algorithm}
}

\def\fuzzyStruckEquation
{
    \begin{align}
        \min_\vec{w} & \half \vec{w} \cdot \vec{w} + C \sum_{i=1}^n \alert{s_i} \xi_i \\
        \text{s.t. } & \alert{s_i} \xi_i \ge 0 \nonumber \\
        & \forall \vec{y} \ne \vec{y}_i : \vec{w} \cdot \delta \vec{\Phi}_i(\vec{y}) \ge
        \loss - \alert{s_i} \xi_i \nonumber
    \end{align}
}

\def\fuzzyStruckDualAlpha
{
    \begin{align}
        \max_\alpha & \sum_{i,\vec{y} \ne \vec{y}_i} \loss \alpha_i^\vec{y} - \half
        \sum_{\substack{i, \vec{y} \ne \vec{y}_i \\ j, \vec{y} \ne \vec{y}_j}} \alpha_i^\vec{y}
        \alpha_j^\vec{\bar{y}} \delta \vec{\Phi}_i( \vec{y} ) \cdot \delta \vec{\Phi}_j(
        \vec{\bar{y}} ) \\
        \text{s.t. } & \forall i, \forall \vec{y} \ne \vec{y}_i : \alpha_i^\vec{y} \ge 0 \nonumber \\
        & \forall i : \sum_{\vec{y} \ne \vec{y}_i} \alpha_i^\vec{y} \le \alert{s_i} C \nonumber
    \end{align}
}

\def\fuzzyStruckDualBeta
{
    \begin{align}
        \max_\beta & - \sum_{i, \vec{y}} \loss \beta_i^\vec{y} - \half \sum_{i, \vec{y}, j,
        \vec{\bar{y}}} \beta_i^\vec{y} \beta_j^\vec{\bar{y}} \vec{\Phi} \left( \vec{x}_i, \vec{y}
        \right) \cdot \vec{\Phi} \left( \vec{x}_j, \vec{\bar{y}} \right) \\
        \text{s.t. } & \forall \vec{y} : \beta_i^\vec{y} \le \begin{cases}
            0 & \vec{y} \ne \vec{y}_i \\
            \alert{s_i} C & \vec{y} = \vec{y}_i
        \end{cases} \nonumber \\
        & \sum_\vec{y} \beta_i^\vec{y} = 0 \nonumber
    \end{align}
}

\def\fuzzyStruckFuzziness
{
    \[ s_i = \frac{\vec{p}_t \cap \vec{p}_i}{\vec{p}_t \cup \vec{p}_i} \]
}

\def\fuzzyStruckWeightChange
{
    \begin{align*}
        \vec{\bar{w}} &= \vec{w} - \beta_r^\vec{y} \vec{\Phi} \left( \vec{x}_r, \vec{y} \right) +
        \beta_r^\vec{y} \vec{\Phi} \left( \vec{x}_r, \vec{y}_r \right) \\
        &= \vec{w} + \beta_r^\vec{y} \left[ \vec{\Phi} \left( \vec{x}_r, \vec{y}_r \right) -
        \vec{\Phi} \left( \vec{x}_r, \vec{y} \right) \right] \\
        \|\Delta \vec{w}\|^2 &= \beta_r^\vec{y} \left[ \vec{\Phi} \left( \vec{x}_r, \vec{y}_r \right) -
        \vec{\Phi} \left( \vec{x}_r, \vec{y} \right) \right]
    \end{align*}
}

\def\fuzzyStruckSmo
{
    \begin{algorithm}%[H]
        \DontPrintSemicolon
        \KwIn{\(i, \vec{y}_-, \vec{y}_+\)}
        \Begin(SMO Step)
        {
            \(\lambda^u = \frac{g_i(\vec{y}_+) - g_i(\vec{y}_-)}{K_{++} + K_{--} -2K_{+-}}\)\;
            \(\lambda = max(0, min(\lambda^u, \alert{s_i} C \delta (\vec{y}_+, \vec{y}_-) - \beta_i^{\vec{y}_+})) \)\;
            \(\beta_i^{\vec{y}_+} \gets \beta_i{\vec{y}_+} + \lambda\)\;
            \(\beta_i^{\vec{y}_-} \gets \beta_i{\vec{y}_-} - \lambda\)\;
            \ForEach{\((\vec{x}_j, \vec{y}) \in \mathcal{S}\)}
            {
                \(K_0 = \vec{\Phi} (\vec{x}_j, \vec{y}) \cdot \vec{\Phi} (\vec{x}_i, \vec{y}_+)\)\;
                \(K_1 = \vec{\Phi} (\vec{x}_j, \vec{y}) \cdot \vec{\Phi} (\vec{x}_i, \vec{y}_-)\)\;
                \(g_j(\vec{y}) \gets g_j(\vec{y}) - \lambda (K_0 - K_1)\)\;
            }
        }
    \end{algorithm}
}
